![[Pasted image 20250626202259.png]]

Как мы знаем $$\vec{F}_{тр}=-\beta \vec{v}$$

Пишем уравнение движения $$m \frac{d\vec{v}}{dt}=m\vec{g}+\vec{F}_{Тр}$$
$$\begin{matrix}
\implies m \dfrac{d\vec{v}}{dt}=m\vec{g}-\beta\vec{v} \\
\dfrac{d\vec{v}}{dt}=\vec{g}-\alpha \vec{v}
\end{matrix}$$

$$\left\{\begin{matrix}
\dfrac{dv_{x}}{dt}=0-\alpha v_{x} \\
\dfrac{dv_{y}}{dt}=g-\alpha v_{y}
\end{matrix}\right. \implies \left\{\begin{matrix}
\dfrac{dv_{x}}{dt}=\alpha v_{x} \\
\dfrac{dv_{y}}{dt}=g-\alpha v_{y}
\end{matrix}\right.$$

Давайте теперь искать скорость.

Начнем с $v_{x}$:

$$\int_{v_{0}\cos \theta}^{v_{x}(t)} \dfrac{dv_{x}}{v_{x}}=-\alpha \int_{0}^{t}dt$$
$$\ln v_{x}(t) \mid^{v_{x}(t)}_{v_{o}\cos \theta}=e^{-\alpha t}$$
$$
\implies v_{x}(t)=v_{x}(t)=v_{0}\cos \theta e^{-\alpha t}$$
$$v_{x}(t)=\frac{dx}{dt}\implies \int_{0}^{L} dx=v_{0}\cos \theta \int_{0}^{t_{под}}e^{-\alpha t}dt$$
$$\boxed{L=\frac{v_{0}\cos \theta}{\alpha}(1-e^{\alpha t_{под}})}$$

$$\frac{dv_{y}}{dt}=-g-\alpha v_{y}=-\alpha\left( v_{y}+\frac{g}{\alpha} \right)$$
$$\int_{v_{0}\sin \theta}^{0} \frac{dv_{y}}{v_{y}+\frac{g}{\alpha}}=-\alpha \int_{0}^{t_{под}}dt$$
$$\implies \ln\left( \frac{g}{\alpha} \right)-\ln\left( v_{0}\sin \theta+\frac{g}{\alpha} \right)=-\alpha t_{под}$$
